Gt3/JEq/Lsv.lean
@@ -55,9 +55,7 @@ theorem Ctx.JEq.lst_cf_univ {Γ : Ctx} {n : ℕ} {A a a'} {B B' : Tm 1} {L : Fin
   (ha : Ctx.JEq Γ A a a') : JEq Γ (.univ n) (B.lst a) (B'.lst a') :=
   have ⟨m, hA⟩ := ha.regular;
   have hAB : Ctx.JEq Γ (.pi A (.univ n)) (.abs A B) (.abs A B') :=
-    .abs hA
-      (fun x hx => by convert JEq.univ (hB x hx).ok using 0; rw[Tm.open_univ])
-      (fun x hx => by convert hB x hx using 0 ; rw [Tm.open_univ])
+    .abs hA (fun x hx => by convert hB x hx using 0 ; rw [Tm.open_univ])
   have app_eq
     : Ctx.JEq Γ (.univ n) (.app (.abs A B) a) (.app (.abs A B') a')
     := .app' (fun x hx => by convert JEq.univ (ℓ := n) (.cons hA.ok hx ⟨_, hA⟩) <;> simp) hA
@@ -131,16 +129,16 @@ theorem Ctx.JEq.lst_cf {Γ : Ctx} {A a a'} {B b b' : Tm 1} {L : Finset String}
     := fun x hx => by simp at hx; exact hb x hx.left
   have app_eq
     : Ctx.JEq Γ (B.lst a) (.app (.abs A b) a) (.app (.abs A b') a')
-    := .app_r (fun x hx => (hb x hx).regular) (.abs hA hB hb) ha hB'.lhs_is_ty
+    := .app_r (fun x hx => (hb x hx).regular) (.abs hA hb) ha hB'.lhs_is_ty
   have hbl := (fun x hx => (hb x hx).lhs_ty')
   have hba := (JEq.lst_cf₁ hbl ha.lhs_ty')
   have hba : Ctx.JEq Γ (B.lst a) (.app (.abs A b) a) (b.lst a)
-    := .beta_app' (.abs hA hB hbl) ha.lhs_ty' app_eq.lhs_ty' hba hba
+    := .beta_app' (.abs hA hbl) ha.lhs_ty' app_eq.lhs_ty' hba hba
   have hbr := (fun x hx => (hb x hx).rhs_ty')
   have hba' := (JEq.lst_cf₁ hbr ha.rhs_ty')
   have hba' : Ctx.JEq Γ (B.lst a') (.app (.abs A b') a') (b'.lst a')
     :=.beta_app'
-      (.abs hA hB hbr) ha.rhs_ty' (app_eq.rhs_ty'.cast ⟨_, hB'⟩)
+      (.abs hA hbr) ha.rhs_ty' (app_eq.rhs_ty'.cast ⟨_, hB'⟩)
       hba' hba'
   exact hba.symm.trans (app_eq.trans (hB'.symm.cast' hba'))
 
