Gt3/RwEq/Erase.lean
@@ -1,0 +1,287 @@
+import Gt3.RwEq.Basic
+import Gt3.HasTy.Inversion
+
+def Ctx.KJEq (Γ : Ctx) (A a b : OTm) : Prop := JEq Γ (A.clamp 0) (a.clamp 0) (b.clamp 0)
+
+theorem Ctx.KJEq.get {Γ A a b} (h : KJEq Γ A a b)
+  : JEq Γ (A.clamp 0) (a.clamp 0) (b.clamp 0) := h
+
+def Ctx.KIsTy (Γ : Ctx) (a : OTm) : Prop := IsTy Γ (a.clamp 0)
+
+theorem Ctx.KIsTy.univ {Γ ℓ} (h : Ok Γ) : KIsTy Γ (.univ ℓ) := IsTy.univ h
+
+theorem Ctx.KIsTy.empty {Γ} (h : Ok Γ) : KIsTy Γ .empty := IsTy.empty h
+
+theorem Ctx.KIsTy.unit {Γ} (h : Ok Γ) : KIsTy Γ .unit := IsTy.unit h
+
+theorem Ctx.KIsTy.nats {Γ} (h : Ok Γ) : KIsTy Γ .nats := IsTy.nats h
+
+theorem Ctx.KIsTy.get {Γ a} (h : KIsTy Γ a)
+  : IsTy Γ (a.clamp 0) := h
+
+def Ctx.KTyEq (Γ : Ctx) (a b : OTm) : Prop := TyEq Γ (a.clamp 0) (b.clamp 0)
+
+theorem Ctx.KTyEq.get {Γ A B} (h : KTyEq Γ A B)
+  : TyEq Γ (A.clamp 0) (B.clamp 0) := h
+
+def Ctx.KIsWf (Γ : Ctx) (a : OTm) : Prop := IsWf Γ (a.clamp 0)
+
+theorem Ctx.KIsWf.lc {Γ a} (h : KIsWf Γ a) : a.bvi = 0 := by convert h.valid.otm_bvi using 0; simp
+
+theorem Ctx.KIsTy.wf {Γ A} (h : KIsTy Γ A) : KIsWf Γ A := h.get.wf
+
+theorem Ctx.KIsTy.lc {Γ A} (h : KIsTy Γ A) : A.bvi = 0 := h.wf.lc
+
+theorem Ctx.KIsWf.univ {Γ ℓ} (h : Ok Γ) : KIsWf Γ (.univ ℓ) := (IsTy.univ h).wf
+
+theorem Ctx.KIsWf.empty {Γ} (h : Ok Γ) : KIsWf Γ .empty := (IsTy.empty h).wf
+
+theorem Ctx.KIsWf.unit {Γ} (h : Ok Γ) : KIsWf Γ .unit := (IsTy.unit h).wf
+
+theorem Ctx.KIsWf.null {Γ} (h : Ok Γ) : KIsWf Γ .null := (JEq.null h).lhs_is_wf
+
+theorem Ctx.KIsWf.nats {Γ} (h : Ok Γ) : KIsWf Γ .nats := (IsTy.nats h).wf
+
+theorem Ctx.KIsWf.zero {Γ} (h : Ok Γ) : KIsWf Γ .zero := (JEq.zero h).lhs_is_wf
+
+theorem Ctx.KIsWf.get {Γ a} (h : KIsWf Γ a)
+  : IsWf Γ (a.clamp 0) := h
+
+def Ctx.KHasTy (Γ : Ctx) (A a : OTm) : Prop := HasTy Γ (A.clamp 0) (a.clamp 0)
+
+theorem Ctx.KHasTy.get {Γ A a} (h : KHasTy Γ A a)
+  : HasTy Γ (A.clamp 0) (a.clamp 0) := h
+
+theorem Ctx.KHasTy.is_wf {Γ A a} (h : KHasTy Γ A a) : KIsWf Γ a := h.get.is_wf
+
+theorem Ctx.KHasTy.regular {Γ A a} (h : KHasTy Γ A a) : KIsTy Γ A := h.get.regular
+
+def Ctx.KWEq (Γ : Ctx) (a b : OTm) : Prop := WfEq Γ (a.clamp 0) (b.clamp 0)
+
+theorem Ctx.KWEq.get {Γ a b} (h : KWEq Γ a b)
+  : WfEq Γ (a.clamp 0) (b.clamp 0) := h
+
+inductive Ctx.KEq (Γ : Ctx) : OTm → OTm → Prop
+  | fv (x) : KEq Γ (.fv x) (.fv x)
+  | bv (i) : KEq Γ (.bv i) (.bv i)
+  | univ (ℓ) : KEq Γ (.univ ℓ) (.univ ℓ)
+  | empty : KEq Γ .empty .empty
+  | unit : KEq Γ .unit .unit
+  | null : KEq Γ .null .null
+  | eqn {a a' b b'} : KEq Γ a a' → KEq Γ b b' → KEq Γ (.eqn a b) (.eqn a' b')
+  | pi {A A' B B'} : KEq Γ A A' → KEq Γ B B' → KEq Γ (.pi A B) (.pi A' B')
+  | sigma {A A' B B'} : KEq Γ A A' → KEq Γ B B' → KEq Γ (.sigma A B) (.sigma A' B')
+  | abs {A A' b b'} : KEq Γ A A' → KEq Γ b b' →
+    KEq Γ (.abs A b) (.abs A' b')
+  | app {f f' a a'} : KEq Γ f f' → KEq Γ a a' → KEq Γ (.app f a) (.app f' a')
+  | pair {a a' b b'} : KEq Γ a a' → KEq Γ b b' →
+    KEq Γ (.pair a b) (.pair a' b')
+  | fst {p p'} : KEq Γ p p' → KEq Γ (.fst p) (.fst p')
+  | snd {p p'} : KEq Γ p p' → KEq Γ (.snd p) (.snd p')
+  | dite {φ φ' l l' r r'} : KEq Γ φ φ' → KEq Γ l l' → KEq Γ r r' →
+    KEq Γ (.dite φ l r) (.dite φ' l' r')
+  | trunc {A A'} : KEq Γ A A' → KEq Γ (.trunc A) (.trunc A')
+  | choose {A A' φ φ'} : KEq Γ A A' → KEq Γ φ φ' → KEq Γ (.choose A φ) (.choose A' φ')
+  | nats : KEq Γ .nats .nats
+  | zero : KEq Γ .zero .zero
+  | succ {n n'} : KEq Γ n n' → KEq Γ (.succ n) (.succ n')
+  | natrec {C C' s  s' z  z' n n'} : KEq Γ C C' → KEq Γ s s' →
+    KEq Γ z z' → KEq Γ n n' → KEq Γ (.natrec C s z n) (.natrec C' s' z' n')
+  | has_ty {A A' a a'} : KEq Γ A A' → KEq Γ a a' → KEq Γ (.has_ty A a) (.has_ty A' a')
+  | invalid : KEq Γ .invalid .invalid
+  | wf_clamp {a b} : KWEq Γ a b → KEq Γ a b
+  | trans {a b c} : KEq Γ a b → KEq Γ b c → KEq Γ a c
+
+theorem Ctx.RwEq.erase {k} {Γ} {a b : Tm k} (h : RwEq Γ a b) : KEq Γ a.erase b.erase := by
+  induction h with
+  | wf_clamp h => apply KEq.wf_clamp; convert h; simp only [KWEq, Tm.erase_clamp]
+  | trans => apply KEq.trans <;> assumption
+  | _ => constructor <;> assumption
+
+theorem Ctx.KEq.clamp {Γ} {a b : OTm} (h : KEq Γ a b) (k : ℕ) : RwEq Γ (a.clamp k) (b.clamp k) := by
+  induction h generalizing k with
+  | bv => apply RwEq.refl
+  | wf_clamp h => apply RwEq.wf_clamp; convert h; simp [KWEq]
+  | trans => apply RwEq.trans <;> apply_assumption
+  | _ => constructor <;> apply_assumption
+
+theorem Ctx.KEq.clamp_iff {Γ} {a b : OTm} : KEq Γ a b ↔ ∀ k, RwEq Γ (a.clamp k) (b.clamp k) := ⟨
+  fun h => h.clamp,
+  fun h => by convert (h (a.bvi ⊔ b.bvi)).erase <;> rw [OTm.erase_clamp_bvi_le] <;> simp⟩
+
+theorem Ctx.KEq.symm {Γ} {a b : OTm} (h : KEq Γ a b) : KEq Γ b a := by
+  rw [clamp_iff] at *
+  exact (fun k => (h k).symm)
+
+theorem Ctx.KEq.psub {Γ Δ} (h : Γ.PSub Δ) {a b : OTm} (hab : KEq Δ a b) : KEq Γ a b := by
+  rw [clamp_iff] at *
+  exact (fun k => (hab k).psub h)
+
+theorem Ctx.KEq.not_ok {Γ} (hΓ : ¬Ok Γ) {k} {a b : Tm k} (hab : RwEq Γ a b) : a = b
+  := by induction hab with
+  | wf_clamp h => exact (hΓ h.ok).elim
+  | _ => simp only [*]
+
+theorem Ctx.KEq.wk0
+  {Γ} {k} {a b : Tm k} (hab : RwEq Γ a b) {x X} (hx : x ∉ Γ.dv) (hX : X ∈ RwTy Γ)
+  : RwEq (Γ.cons x X) a b
+  := open Classical in
+  if hΓ : Ok Γ then
+    hab.psub (hΓ.psub.skip hx (hX hΓ))
+  else
+    .of_eq (not_ok hΓ hab)
+
+theorem Ctx.KEq.jeq {Γ} {A a b : OTm} (h : KEq Γ a b) (ha : KHasTy Γ A a)
+  : KJEq Γ A a b := (h.clamp 0).lwreq.jeq_or (.inl ha)
+
+theorem Ctx.KEq.has_ty_mp {Γ} {A a b : OTm} (h : KEq Γ a b)
+  (ha : KHasTy Γ A a) : KHasTy Γ A b
+  := (h.jeq ha).rhs_ty
+
+theorem Ctx.KEq.has_ty_iff {Γ} {A a b : OTm} (h : KEq Γ a b)
+  : KHasTy Γ A a ↔ KHasTy Γ A b
+  := ⟨h.has_ty_mp, h.symm.has_ty_mp⟩
+
+theorem Ctx.KEq.ty_eq {Γ} {A B : OTm} (h : KEq Γ A B) (hA : KIsTy Γ A)
+  : KTyEq Γ A B := have ⟨ℓ, hA⟩ := hA; ⟨ℓ, (h.clamp 0).jeq hA.lhs_ty⟩
+
+theorem Ctx.KEq.is_ty {Γ} {A B : OTm} (h : KEq Γ A B) (hA : KIsTy Γ A)
+  : KIsTy Γ B := (h.ty_eq hA).rhs
+
+theorem Ctx.KEq.is_ty_iff {Γ} {A B : OTm} (h : KEq Γ A B)
+  : KIsTy Γ A ↔ KIsTy Γ B := ⟨h.is_ty, h.symm.is_ty⟩
+
+theorem Ctx.KEq.weq {Γ} {a b : OTm} (h : KEq Γ a b) (ha : KIsWf Γ a)
+  : KWEq Γ a b := (h.clamp 0).weq ha
+
+theorem Ctx.KEq.is_wf {Γ} {a b : OTm} (h : KEq Γ a b) (hA : KIsWf Γ a)
+  : KIsWf Γ b := (h.weq hA).rhs
+
+theorem Ctx.KEq.wf_iff {Γ} {a b : OTm} (h : KEq Γ a b)
+  : KIsWf Γ a ↔ KIsWf Γ b := ⟨h.is_wf, h.symm.is_wf⟩
+
+def Ctx.HasTyUnder (Γ : Ctx) (A : Tm 0) (B b : Tm 1) : Prop
+  := ∀ x ∉ Γ.dv, HasTy (Γ.cons x A) (B.open x) (b.open x)
+
+def Ctx.KHasTyUnder (Γ : Ctx) (A B b : OTm) : Prop
+  := ∀ x ∉ Γ.dv, KHasTy (Γ.cons x (A.clamp 0)) (B.open 0 x) (b.open 0 x)
+
+theorem Ctx.KHasTyUnder.get {Γ A B b} (h : KHasTyUnder Γ A B b)
+  : HasTyUnder Γ (A.clamp 0) (B.clamp 1) (b.clamp 1)
+  := by
+  simp only [HasTyUnder]
+  intro x hx
+  convert (h x hx).get <;> simp [OTm.clamp_succ_open]
+
+theorem Ctx.KHasTy.wk0 {Γ A a} (h : KHasTy Γ A a) {x X} (hx : x ∉ Γ.dv) (hX : X ∈ RwTy Γ)
+  : KHasTy (Γ.cons x X) A a
+  := HasTy.wk0 h hx (hX h.ok)
+
+theorem Ctx.KHasTy.under {Γ A B b} (hB : KIsTy Γ A) (h : KHasTy Γ B b)
+  : KHasTyUnder Γ A B b
+  := by
+  intro x hx
+  apply KHasTy.wk0 _ hx (fun _ => hB)
+  convert h <;> rw [OTm.open_bvi] <;> rw [KIsWf.lc]
+  · apply KIsTy.wf; apply KHasTy.regular; assumption
+  · apply KHasTy.is_wf; assumption
+
+theorem Ctx.KIsWf.to_has_ty {Γ A a} (ha : KIsWf Γ (.has_ty A a)) : KHasTy Γ A a := ha.get.to_has_ty
+
+theorem Ctx.KIsWf.to_has_ty_under {Γ A B b} (h : KIsWf Γ (.abs A (.has_ty B b)))
+  : KHasTyUnder Γ A B b
+  := by
+  intro x hx
+  apply IsWf.to_has_ty
+  have ⟨_, h⟩ := h.get;
+  have ⟨_, h⟩ := h.lhs_ty.inner_ty;
+  cases h with
+  | abs hA hB hb =>
+    convert (HasTy.top_quant_exact hb x hx).is_wf
+    simp [OTm.clamp, OTm.clamp_succ_open]
+
+theorem Ctx.KHasTyUnder.param {Γ A B b} (h : KHasTyUnder Γ A B b) : KIsTy Γ A
+  := have ⟨x, hx⟩ := Γ.dv.exists_notMem; (h x hx).ok.ty
+
+theorem Ctx.KHasTy.m_has_ty_wf {Γ A a} (ha : KHasTy Γ A a) : KIsWf Γ (.has_ty A a)
+  := ⟨_, ha.get.m_has_ty.refl⟩
+
+theorem Ctx.KHasTy.wf_iff {Γ A a} : KIsWf Γ (.has_ty A a) ↔ KHasTy Γ A a
+  := ⟨KIsWf.to_has_ty, fun h => (m_has_ty_wf h)⟩
+
+def Ctx.IsWfUnder (Γ : Ctx) (A : Tm 0) (B : Tm 1) : Prop
+  := ∀ x ∉ Γ.dv, IsWf (Γ.cons x A) (B.open x)
+
+def Ctx.IsTyUnder (Γ : Ctx) (A : Tm 0) (B : Tm 1) : Prop
+  := ∀ x ∉ Γ.dv, IsTy (Γ.cons x A) (B.open x)
+
+def Ctx.KIsWfUnder (Γ : Ctx) (A B : OTm) : Prop
+  := ∀ x ∉ Γ.dv, KIsWf (Γ.cons x (A.clamp 0)) (B.open 0 x)
+
+theorem Ctx.KIsWfUnder.param {Γ A B} (h : KIsWfUnder Γ A B) : KIsTy Γ A
+  := have ⟨x, hx⟩ := Γ.dv.exists_notMem; (h x hx).ok.ty
+
+def Ctx.KIsTyUnder (Γ : Ctx) (A B : OTm) : Prop
+  := ∀ x ∉ Γ.dv, KIsTy (Γ.cons x (A.clamp 0)) (B.open 0 x)
+
+theorem Ctx.KIsTyUnder.param {Γ A B} (h : KIsTyUnder Γ A B) : KIsTy Γ A
+  := have ⟨x, hx⟩ := Γ.dv.exists_notMem; (h x hx).ok.ty
+
+theorem Ctx.KHasTyUnder.ty {Γ A B b} (h : KHasTyUnder Γ A B b) : KIsTyUnder Γ A B
+  := fun x hx => (h x hx).regular
+
+theorem Ctx.KIsTyUnder.wf {Γ A B} (h : KIsTyUnder Γ A B) : KIsWfUnder Γ A B
+  := fun x hx => (h x hx).wf
+
+theorem Ctx.KHasTyUnder.is_wf {Γ A B b} (h : KHasTyUnder Γ A B b) : KIsWfUnder Γ A b
+  := fun x hx => (h x hx).is_wf
+
+theorem Ctx.KHasTy.univ {Γ ℓ} (h : Ok Γ) : KHasTy Γ (.univ (ℓ + 1)) (.univ ℓ)
+  := HasTy.univ h
+
+theorem Ctx.KHasTy.empty {Γ ℓ} (h : Ok Γ) : KHasTy Γ (.univ ℓ) .empty
+  := HasTy.empty h
+
+theorem Ctx.KHasTy.unit {Γ ℓ} (h : Ok Γ) : KHasTy Γ (.univ ℓ) .unit
+  := HasTy.unit h
+
+theorem Ctx.KHasTy.nats {Γ} (h : Ok Γ) : KHasTy Γ (.univ 1) .nats
+  := HasTy.nats h
+
+theorem Ctx.KHasTy.pi {Γ A B ℓ}
+  (hA : KHasTy Γ (.univ ℓ) A) (hB : KHasTyUnder Γ A (.univ ℓ) B)
+  (hℓ : 1 ≤ ℓ) : KHasTy Γ (.univ ℓ) (.pi A B)
+  := HasTy.pi
+    hA (fun x hx => by convert (hB x hx).get; simp [OTm.clamp_succ_open])
+    (le_refl ℓ) (le_refl ℓ) hℓ
+
+theorem Ctx.KHasTy.abs {Γ A B b}
+  (hB : KHasTyUnder Γ A B b) : KHasTy Γ (.pi A B) (.abs A b)
+  := HasTy.abs (fun x hx => by convert (hB x hx).get <;> simp [OTm.clamp_succ_open])
+
+--TODO: app
+
+theorem Ctx.KHasTy.sigma {Γ A B ℓ}
+  (hA : KHasTy Γ (.univ ℓ) A) (hB : KHasTyUnder Γ A (.univ ℓ) B)
+  (hℓ : 1 ≤ ℓ) : KHasTy Γ (.univ ℓ) (.sigma A B)
+  := HasTy.sigma
+    hA (fun x hx => by convert (hB x hx).get; simp [OTm.clamp_succ_open])
+    (le_refl ℓ) (le_refl ℓ) hℓ
+
+--TODO: pair
+
+--TODO: fst
+
+--TODO: snd
+
+--TODO: dite, ite, and friends
+
+--TODO: trunc
+
+--TODO: choose
+
+--TODO: succ
+
+--TODO: natrec
+
+--TODO: closure runes
